\documentclass[11pt]{article}

\usepackage{mathtools}
\usepackage{amssymb}
\usepackage[latin1]{inputenc}
\usepackage[margin=0.5in]{geometry}

\everymath{\displaystyle}
\setlength\parindent{0pt}

\begin{document}
\title{Stanford CS 229, Public Course, Problem Set 1}
\date{\today}
\author{Dylan Price}
\maketitle 

% custom commands
\newcommand{\pder}[2]{\frac{\partial#1}{\partial#2}}
\newcommand{\thetaT}[0]{\theta^{T}}
\newcommand{\ith}[1]{#1^{(i)}}
\newcommand{\xith}[0]{\ith{x}}
\newcommand{\yith}[0]{\ith{y}}
\newcommand{\sumitom}[0]{\sum_{i=1}^{m}}


\section{}

\subsection*{a)}

Find the Hessian of the cost function $J(\theta) = \frac{1}{2} \sumitom (\thetaT \xith - \yith)^{2}$

We know that $H_{jk} = \frac{\partial^{2}J(\theta)}{\partial\theta_{j}\theta_{k}}$ \\

First find $\frac{\partial J(\theta)}{\partial\theta_{k}}$,

\begin{align*}
  \pder{J(\theta)}{\theta_{k}} &= \frac{1}{2} \sumitom \pder{}{\theta_{k}} (\thetaT \xith - \yith)^{2} \\
  &= \frac{1}{2} \sumitom 2 (\thetaT \xith - \yith)(\ith{x_{k}}) \\
  &= \sumitom (\thetaT \xith - \yith)(\ith{x_{k}})
\end{align*}

Now find $\frac{\partial^{2}J(\theta)}{\partial\theta_{j}\theta_{k}}$, \\

\begin{align*}
  \frac{\partial^{2}J(\theta)}{\partial\theta_{j}\theta_{k}} &= \pder{}{\theta_{j}} ( \pder{J(\theta)}{\theta_{k}} ) \\
  &= \sumitom \pder{}{\theta_{j}} ((\thetaT \xith - \yith)(\ith{x_{k}})) \\
  &= \sumitom \ith{x_{j}} \ith{x_{k}} \text{ for } 1 \leq j \leq n \text{ and } 1 \leq k \leq n
\end{align*}

Therefore
\begin{align*}
  H &= 
  \begin{bmatrix}
    \sumitom \ith{x_{1}} \ith{x_{1}} & \sumitom \ith{x_{2}} \ith{x_{1}} & \cdots & \sumitom \ith{x_{n}} \ith{x_{1}} \\
    \sumitom \ith{x_{1}} \ith{x_{2}} & \sumitom \ith{x_{2}} \ith{x_{2}} & \cdots & \sumitom \ith{x_{n}} \ith{x_{2}} \\
    \vdots                           & \vdots                           & \ddots & \vdots \\
    \sumitom \ith{x_{1}} \ith{x_{n}} & \sumitom \ith{x_{2}} \ith{x_{n}} & \cdots & \sumitom \ith{x_{n}} \ith{x_{n}} 
  \end{bmatrix}
  \\ &=
  \begin{bmatrix}
    x_{1}^{(1)} & \cdots & x_{1}^{(n)} \\
    \vdots      & \ddots & \vdots \\
    x_{m}^{(1)} & \cdots & x_{m}^{(n)}
  \end{bmatrix}
  \begin{bmatrix}
    x_{1}^{(1)} & \cdots & x_{m}^{(1)} \\
    \vdots      & \ddots & \vdots \\
    x_{1}^{(n)} & \cdots & x_{m}^{(n)}
  \end{bmatrix}
  \\ &= X^{T} X
\end{align*}

\subsection*{b)}

Show that the first iteration of Newton's method gives us $\theta^{*} = (X^{T} X)^{-1} X^{T} \vec{y}$, the solution to our least squares problem. \\

One iteration of Newton's Method: \\
$\theta := \theta - H^{-1} \nabla_{\theta} J(\theta)$ \\
Therefore,

\begin{align*}
  \theta^{*} &= 
  \theta - (X^{T} X)^{-1}
  \begin{bmatrix}
    \pder{J(\theta)}{\theta_{1}} \\
    \vdots \\
    \pder{J(\theta)}{\theta_{m}}
  \end{bmatrix}
  \\ &= 
  \theta - (X^{T} X)^{-1}
  \begin{bmatrix}
    \sumitom ( \ith{x_{1}} \thetaT \xith - \ith{x_{1}} \yith ) \\
    \vdots \\
    \sumitom ( \ith{x_{m}} \thetaT \xith - \ith{x_{m}} \yith )
  \end{bmatrix}
  \\ \text{let $\theta = \vec{0}$ (initialize $\theta$)}
  \\ &= 
  - (X^{T} X)^{-1}
  \begin{bmatrix}
    \sumitom ( - \ith{x_{1}} \yith ) \\
    \vdots \\
    \sumitom ( - \ith{x_{m}} \yith )
  \end{bmatrix}
  \\ &=
  (X^{T} X)^{-1}
  \begin{bmatrix}
    \sumitom ( \ith{x_{1}} \yith ) \\
    \vdots \\
    \sumitom ( \ith{x_{m}} \yith )
  \end{bmatrix}
  \\ &=
  (X^{T} X)^{-1} X^{T} \vec{y}
\end{align*}
  


\section*{2}

\subsection*{a}
See q2/ folder

\subsection*{b}
At low values of $\tau$, the classification boundaries are clustered around the positive training examples. As you increase $\tau$, these boundaries begin to merge into bigger areas, i.e. the classification boundaries look less 'local' to the positive training examples. At high values of $\tau$, the classification boundary is essentially a straight line dividing positive and negative classes. \\

The decision boundary of unweighted logistic regression would look like the plots with the highest values of $\tau$. This is because as $\tau$ approaches infinity, the weight function $w^{(i)}$ goes to 1 for every training example, making the regression unweighted (that is, every training example gets the same weight).

\section*{3}

\subsection*{a)}

\begin{align*}
    J(\theta) &= \frac{1}{2} \sumitom \sum_{j=1}^p ((\thetaT \xith)_j - y_j^{(i)})^2 \\
              &= \frac{1}{2} \sumitom (\thetaT \xith - y^{(i)})^T (\thetaT \xith - y^{(i)}) \\
              & \text{Let $\vec{1}$ be a vector of all ones.} \\
              &= \frac{1}{2} \vec{1}^T (X \theta - Y)^T (X \theta - Y) \vec{1} \\
\end{align*}

\subsection*{b)}

\begin{align*}
    J(\theta) &= \frac{1}{2} \vec{1}^T (X \theta - Y)^T (X \theta - Y) \vec{1} \\
              &= \frac{1}{2} \vec{1}^T ((X \theta)^T - Y^T) (X \theta - Y) \vec{1} \\
              &= \frac{1}{2} \vec{1}^T (\thetaT X^T - Y^T) (X \theta - Y) \vec{1} \\
              &= \frac{1}{2} \vec{1}^T (\thetaT X^T X \theta - \thetaT X^T Y - Y^T X \theta + Y^T Y) \vec{1} \\
              &= \frac{1}{2} \vec{1}^T \thetaT X^T X \theta \vec{1} - \frac{1}{2} \vec{1}^T \thetaT X^T Y \vec{1} - \frac{1}{2} \vec{1}^T Y^T X \theta \vec{1} + \frac{1}{2} \vec{1}^T Y^T Y \vec{1} \\
\end{align*}

\begin{align*}
    \Delta_\theta J(\theta) &= \frac{1}{2} * 2 X^T X \theta - \frac{1}{2} X^T Y - \frac{1}{2} (Y^T X)^T \\
                            &= X^T X \theta - X^T Y
\end{align*}

\begin{align*}
    0            &= X^T X \theta - X^T Y \\
    X^T X \theta &= X^T Y \\
    \theta       &= (X^T X)^{-1} X^T Y \\
\end{align*}

\subsection*{c)}

Consider the multivariate model $\yith = \thetaT \xith$
\begin{align*}
    \yith = \thetaT \xith = 
    \begin{bmatrix}
        \theta_{1,1} & \theta_{1,2} & \cdots & \theta_{1,n} \\
        \theta_{2,1} & \theta_{2,2} &        &              \\
        \vdots       &              & \ddots &              \\
        \theta_{p,1} &              &        & \theta_{p,n} \\
    \end{bmatrix}
    \begin{bmatrix}
        \xith_1 \\
        \xith_2 \\
        \vdots \\
        \xith_n \\
    \end{bmatrix}
    =
    \begin{bmatrix}
        \theta_{1,1} \xith_1 & \theta_{1,2} \xith_2 & \cdots & \theta_{1,n} \xith_n \\
        \theta_{2,1} \xith_1 & \theta_{2,2} \xith_2 &        &                      \\
        \vdots               &                      & \ddots &                      \\
        \theta_{p,1} \xith_1 &                      &        & \theta_{p,n} \xith_n \\
    \end{bmatrix}
    =
    \begin{bmatrix}
        \theta_1^T \xith \\
        \theta_2^T \xith \\
        \vdots         \\
        \theta_p^T \xith \\
    \end{bmatrix}
    =
    \begin{bmatrix}
        \yith_1 \\
        \yith_2 \\
        \vdots  \\
        \yith_p \\
    \end{bmatrix}
\end{align*}

Therefore each row of this multivariate model corresponds to an equation of the form $\yith_j = \thetaT_j \xith$.

\section*{4}

\subsection*{a)}

\begin{align*}
    \ell(\varphi) &= \log \prod_{i=1}^m P(\xith, \yith; \varphi) \\
                  &= \log \prod_{i=1}^m P(\yith) P(\xith | \yith) \\
                  &= \sumitom \log P(\yith) P(\xith | \yith) \\
                  &= \sumitom [ \log P(\yith) + \log \prod_{j=1}^n ( \phi_{j|\yith})^{\xith_j} (1 - \phi_{j|\yith})^{1 - \xith_j} ] \\
                  &= \sumitom [ \log P(\yith) + \sum_{j=1}^n ( \log(\phi_{j|\yith})^{\xith_j} + \log (1 - \phi_{j|\yith})^{1 - \xith_j}) ] \\
                  &= \sumitom [ \log P(\yith) + \sum_{j=1}^n ( \xith_j \log(\phi_{j|\yith}) + (1 - \xith_j) \log (1 - \phi_{j|\yith})) ] \\
                  &= \sumitom [ (\yith \log \phi_y + (1 - \yith) \log (1 - \phi_y) + \sum_{j=1}^n ( \xith_j \log(\phi_{j|\yith}) + (1 - \xith_j) \log (1 - \phi_{j|\yith})) ] \\
\end{align*}

\subsection*{b)}

First find $\phi_y$
\begin{align*}
    \nabla_{\phi_y} \ell(\varphi) &= \sumitom [ \yith \frac{1}{\phi_y} - (1 - \yith) \frac{1}{1 - \phi_y} ] \\
\end{align*}
\begin{align*}
    0               &= \sumitom [ \frac{\yith}{\phi_y} - \frac{1 - \yith}{1 - \phi_y} ] \\
                    &= \sumitom [ \yith ( 1 - \phi_y) - (1 - \yith) \phi_y ] \\
                    &= \sumitom [ \yith - \yith \phi_y - (\phi_y - \yith \phi_y) ] \\
                    &= \sumitom [ \yith - \yith \phi_y - \phi_y + \yith \phi_y ] \\
                    &= \sumitom [ \yith - \phi_y ] \\
    \sumitom \phi_y &= \sumitom \phi_y \\
    m \phi_y        &= \sumitom \yith \\
    \phi_y          &= \frac{\sumitom \yith}{m} = \sumitom \frac{1\{\yith = 1\}}{m}
\end{align*}

Now find $\phi_{j|y=0}$ and $\phi_{j|y=1}$

\begin{align*}
    \nabla_{\phi_{j|\yith}} \ell(\varphi) = &\nabla_{\phi_{j|\yith}} \sumitom [ (\yith \log \phi_y + (1 - \yith) \log (1 - \phi_y) ] + \\
                                            &\nabla_{\phi_{j|\yith}} \sumitom [ \sum_{j=1}^n [ ( \xith_j \log(\phi_{j|\yith}) + (1 - \xith_j) \log (1 - \phi_{j|\yith})) ] ] \\
\end{align*}

We can drop the first term (the one containing references to $\phi_y$) since its gradient with respect to $\phi_{j|\yith}$ is 0. \\
We can also drop $\sum_{j=1}^n$ from the second term because we are taking the gradient with respect to a single $\phi_{j|\yith}$.

\begin{align*}
    &= \nabla_{\phi_{j|\yith}} \sumitom [ \xith \log \phi_{j|\yith} + (1 - \xith) \log (1 - \phi_{j|\yith}) ] \\
    &= \sumitom [ \xith \frac{1}{\phi_{j|\yith}} - (1 - \xith) \frac{1}{1 - \phi_{j|\yith}} ] \\
\end{align*}

\begin{align*}
    0                       &= \sumitom [ \xith \frac{1}{\phi_{j|\yith}} - (1 - \xith) \frac{1}{1 - \phi_{j|\yith}} ] \\
                            &= \sumitom [ \xith ( 1 - \phi_{j|\yith}) - (1 - \xith) \phi_{j|\yith} ] \\
                            &= \sumitom [ \xith - \phi_{j|\yith} ] \\
    \sumitom \phi_{j|\yith} &= \sumitom \xith \\
    \sumitom \phi_{j|y=0} 1\{\yith=0\} &= \sumitom \xith 1\{\yith=0\} \\
    \phi_{j|y=0} &= \frac{\sumitom \xith 1\{\yith=0\}}{\sumitom 1\{\yith=0\}} = \frac{\sumitom 1\{\xith=1 \land \yith=0\}}{\sumitom 1\{\yith=0\}} \\
    \text{Similarly,} \\
    \phi_{j|y=1} &= \frac{\sumitom 1\{\xith=1 \land \yith=1\}}{\sumitom 1\{\yith=1\}} \\
\end{align*}

\subsection*{c)}

We predict $y=1$ when $P(y=1|x) \geq P(y=0|x)$ \\

$P(y=1|x) \geq P(y=0|x)$ \\

$P(y=1|x) - P(y=1|x) \geq 0$ \\

By Bayes Rule: \\

$\frac{P(x|y=1)P(y=1)}{\sum_{a \in Val(y)} P(x|y=a)P(y=a)} - \frac{P(x|y=0)P(y=0)}{\sum_{a \in Val(y)} P(x|y=a)P(y=a)} \geq 0 \\\\\\$

Substituting in the equations from the beginning of the problem (and combining the denominator): \\

$\frac{\phi_y \prod_{j=1}^n (\phi_{j|y=1})^{x_j} (1 - \phi_{j|y=1})^{1-x_j} - (1 - \phi_y) \prod_{j=1}^n (\phi_{j|y=0})^{x_j} (1 - \phi_{j|y=0})^{1 - x_j}}{\phi_y \prod_{j=1}^n (\phi_{j|y=1})^{x_j}(1 - \phi_{j|y=1})^{1-x_j} + (1 - \phi_y) \prod_{j=1}^n (\phi_{j|y=0})^{x_j}(1-\phi_{j|y=0})^{1-x_j}} \geq 0 \\\\\\$ 

$\phi_y \prod_{j=1}^n (\phi_{j|y=1})^{x_j} (1 - \phi_{j|y=1})^{1-x_j} - (1 - \phi_y) \prod_{j=1}^n (\phi_{j|y=0})^{x_j} (1 - \phi_{j|y=0})^{1 - x_j} \geq 0 \\$ 

$\phi_y \prod_{j=1}^n (\phi_{j|y=1})^{x_j} (1 - \phi_{j|y=1})^{1-x_j} \geq (1 - \phi_y) \prod_{j=1}^n (\phi_{j|y=0})^{x_j} (1 - \phi_{j|y=0})^{1 - x_j} \\$

$\log \phi_y + \sum_{j=1}^n x_j \log \phi_{j|y=1} + \sum_{j=1}^n (1-x_j) \log (1 - \phi_{j|y=1}) \geq \log (1 - \phi_y) + \sum_{j=1}^n x_j \log \phi_{j|y=0} + \sum_{j=1}^n (1-x_j) \log (1 - \phi_{j|y=0})$

\begin{align*}
    \log \phi_y - \log (1 - \phi_y) &+ \sum_{j=1}^n x_j \log \phi_{j|y=1} + \sum_{j=1}^n \log (1 - \phi_{j|y=1}) - \sum_{j=1}^n x_j \log (1 - \phi_{j|y=1}) \\
                                    &- \sum_{j=1}^n x_j \log \phi_{j|y=0} - \sum_{j=1}^n \log (1 - \phi_{j|y=0}) + \sum_{j=1}^n x_j \log (1 - \phi_{j|y=0}) \geq 0 \\
    \log \phi_y - \log (1 - \phi_y) &+ \sum_{j=1}^n \log (1 - \phi_{j|y=1}) - \sum_{j=1}^n \log (1 - \phi_{j|y=0}) \\
                                    &+ \sum_{j=1}^n x_j [ \log \phi_{j|y=1} - \log (1 - \phi_{j|y=1}) - \log \phi_{j|y=0} + \log ( 1 - \phi_{j|y=0})] \geq 0 \\
\end{align*}
define $\theta \in \mathbb{R}^{n+1}$ as 
$
\begin{bmatrix}
    \theta_0 \\
    \theta_1 \\
    \vdots \\
    \theta_n
\end{bmatrix}
$ \\

let $\theta_0 = \log \phi_y - \log (1 - \phi_y) + \sum_{j=1}^n \log (1-\phi_{j|y=1}) - \sum_{j=1}^n \log (1-\phi_{j|y=0})$ \\
let $\theta_1 = \log \phi_{1|y=1} - \log (1-\phi_{1|y=1}) - \log \phi_{1|y=0} + \log (1 - \phi_{1|y=0})$ \\
let $\theta_2 = \log \phi_{2|y=1} - \log (1-\phi_{2|y=1}) - \log \phi_{2|y=0} + \log (1 - \phi_{2|y=0})$ \\
... \\
let $\theta_n = \log \phi_{n|y=1} - \log (1-\phi_{n|y=1}) - \log \phi_{n|y=0} + \log (1 - \phi_{n|y=0})$ \\

then the above inequality can be rewritten as \\

$\theta_0 + \theta_1 x_1 + \theta_2 x_2 + ... + \theta_n x_n \geq 0$ \\

$\thetaT \begin{bmatrix} 1 \\ x \\ \end{bmatrix} \geq 0$ \\

\section*{5}

\subsection*{a)}

\begin{align*}
    P(y;\phi) &= (1-\phi)^{y-1} \phi \\
              &= \exp(\log[(1-\phi)^{y-1} \phi]) \\
              &= \exp ( (y-1) \log(1-\phi) + \log\phi ) \\
              &= \exp ( \log(1-\phi) y - \log(1-\phi) + \log \phi ) \\
              &= \exp ( \log(1-\phi) y - (\log(1-\phi) - \log \phi ) \\
              &= \exp ( \log(1-\phi) y - \log(\frac{1-\phi}{\phi}) ) \\
\end{align*}

We can see this is exponential family with \\
$\eta = \log(1-\phi)$ \\
$T(y) = y$ \\
$a(\eta) = \log(\frac{1-\phi}{\phi})$ \\
$b(y) = 1$ \\

Solving $\eta = \log(1-\phi)$ for $\phi$ and substituting into $a(\eta)$, we can find $a(\eta)$ in terms of $\eta$:
\begin{align*}
    \eta       &= \log(1-\phi) \\
    e^{\eta}   &= 1-\phi \\
    \phi       &= 1 - e^{\eta} \\
    \\
    a(\eta) &= \log \frac{1-(1-e^\eta)}{1-e^\eta} \\
    a(\eta) &= \log \frac{e^\eta}{1-e^\eta} \\
\end{align*}

\subsection*{b)}

\begin{align*}
    g(\eta) &= E[T(y);\eta] \\
            &= E[y] \\
            &= \frac{1}{\phi} \\
            &= \frac{1}{1-e^\eta} \\
\end{align*}

\subsection*{c)}

Since $\eta$ is linearly related to $x$, $\eta = \thetaT x$ for some $\theta \in \mathbb{R}^n$ and $\phi = 1 - e^{\thetaT x}$.
\begin{align*}
    P(\yith|\xith;\phi)        &= \exp(\log(1-\phi)\yith - \log(\frac{1-\phi}{\phi})) \\
    P(\yith|\xith;\theta)      &= \exp(\log(1 - (1-e^{\thetaT \xith}))\yith - \log(\frac{1-(1-e^{\thetaT \xith})}{1 - e^{\thetaT \xith}})) \\
    P(\yith|\xith;\theta)      &= \exp(\log(e^{\thetaT \xith})\yith - \log(\frac{e^{\thetaT \xith}}{1 - e^{\thetaT \xith}})) \\
    \log P(\yith|\xith;\theta) &= \log(e^{\thetaT \xith})\yith - \log(\frac{e^{\thetaT \xith}}{1 - e^{\thetaT \xith}}) \\
                               &= \thetaT \xith \yith - ( \log e^{\thetaT \xith} - \log (1 - e^{\thetaT \xith})) \\
                               &= \thetaT \xith \yith - \thetaT \xith + \log (1 - e^{\thetaT \xith}) \\
\end{align*}

\begin{align*}
    \pder{}{\theta_j} \log P(\yith|\xith;\theta) &= \xith_j \yith - \xith_j - \frac{\xith_j e^{\thetaT \xith}}{1 - e^{\thetaT \xith}} \\
        &= \xith_j \yith - \frac{\xith_j(1-e^{\thetaT \xith}) + \xith_j e^{\thetaT \xith}}{1 - e^{\thetaT \xith}} \\
        &= \xith_j \yith - \frac{\xith_j}{1 - e^{\thetaT \xith}} \\
        &= (\yith - \frac{1}{1-e^{\thetaT \xith}}) \xith_j \\
\end{align*}

So the stochastic gradient ascent update rule is $\theta_j := \theta_j + \alpha (\yith - \frac{1}{1 - e^{\thetaT \xith}}) \xith_j$ \\

\end{document}

